SeparationLogic/Sound_Upwards.v
@@ -5,7 +5,7 @@ Require Import Logic.PropositionalLogic.Syntax.
 Require Import Logic.SeparationLogic.Syntax.
 Require Import Logic.PropositionalLogic.KripkeSemantics.
 Require Import Logic.SeparationLogic.SeparationAlgebra.
-Require Import Logic.SeparationLogic.UpwardsSemantics.
+Require Import Logic.SeparationLogic.Semantics. Import Logic.SeparationLogic.Semantics.UpwardsSemantics.
 Require Import Logic.PropositionalLogic.IntuitionisticPropositionalLogic.
 Require Import Logic.SeparationLogic.SeparationLogic.
 
@@ -143,7 +143,7 @@ Proof.
   exists m0, m1, m2; auto.
 Qed.
 
-Lemma sound_sepcon_emp {L: Language} {nL: NormalLanguage L} {pL: PropositionalLanguage L} {SL: SeparationLanguage L} {uSL: UnitarySeparationLanguage L} {MD: Model} {kMD: KripkeModel MD} (M: Kmodel) {kiM: KripkeIntuitionisticModel MD M} {SA: SeparationAlgebra MD M} {USA: UnitarySeparationAlgebra MD M} {uSA: UpwardsClosedSeparationAlgebra MD M} {nUSA: NormalUnitarySeparationAlgebra MD M} {SM: Semantics L MD} {kiSM: KripkeIntuitionisticSemantics L MD M SM} {usSM: UpwardsSemantics L MD M SM} {uUsSM: UnitaryUpwardsSemantics L MD M SM}:
+Lemma sound_sepcon_emp {L: Language} {nL: NormalLanguage L} {pL: PropositionalLanguage L} {SL: SeparationLanguage L} {uSL: UnitarySeparationLanguage L} {MD: Model} {kMD: KripkeModel MD} (M: Kmodel) {kiM: KripkeIntuitionisticModel MD M} {SA: SeparationAlgebra MD M} {USA: UnitarySeparationAlgebra MD M} {uSA: UpwardsClosedSeparationAlgebra MD M} {nUSA: NormalUnitarySeparationAlgebra MD M} {SM: Semantics L MD} {kiSM: KripkeIntuitionisticSemantics L MD M SM} {usSM: UpwardsSemantics L MD M SM} {UsSM: UnitarySemantics L MD M SM}:
   forall x: expr,
     forall m, KRIPKE: M, m |= x * emp <--> x.
 Proof.
@@ -157,12 +157,9 @@ Proof.
     rewrite sat_sepcon in H0.
     destruct H0 as [m'' [m' [u [? [? [? ?]]]]]].
     rewrite sat_emp in H2.
-    destruct H2 as [u' [? ?]].
-    destruct (join_Korder_up _ _ _ m' u' H0) as [m''' [? ?]]; [reflexivity | auto |].
-    apply join_comm in H4.
-    rewrite unit_spec in H3.
-    apply H3 in H4.
-    eapply sat_mono; eauto.
+    apply join_comm in H0.
+    rewrite unit_spec in H2.
+    apply H2 in H0.
     eapply sat_mono; eauto.
     eapply sat_mono; eauto.
   + rewrite sat_impp; intros.
@@ -173,8 +170,7 @@ Proof.
     - reflexivity.
     - apply join_comm; auto.
     - rewrite sat_emp.
-      exists u; split; auto.
-      reflexivity.
+      auto.
 Qed.
 
 Lemma sound_sepcon_elim {L: Language} {nL: NormalLanguage L} {pL: PropositionalLanguage L} {SL: SeparationLanguage L} {MD: Model} {kMD: KripkeModel MD} (M: Kmodel) {kiM: KripkeIntuitionisticModel MD M} {SA: SeparationAlgebra MD M} {GC: GarbageCollectSeparationAlgebra MD M} {SM: Semantics L MD} {kiSM: KripkeIntuitionisticSemantics L MD M SM} {usSM: UpwardsSemantics L MD M SM}:
